Updated CSP, ACP and RP

theories/theories/utp_csp.thy
@@ -1,5 +1,5 @@
 (******************************************************************************)
-(* Project: Mechanisation of the UTP                                          *)
+(* Project: Mechanation of the UTP                                          *)
 (* File: utp_csp.thy                                                          *)
 (* Authors: Samuel Canham and Simon Foster, University of York                *)
 (******************************************************************************)
@@ -11,93 +11,101 @@ imports
   utp_designs
   utp_theory
   utp_reactive
+  utp_acp
 begin
 
 definition J_pred_rea :: "'VALUE WF_PREDICATE" ("J\<^bsub>rea\<^esub>") where
-"J\<^bsub>rea\<^esub> \<equiv> (ok \<Rightarrow>p ok') \<and>p II (REL_VAR - OKAY)"
+"J\<^bsub>rea\<^esub> \<equiv> `(ok \<Rightarrow> ok') \<and> II\<^bsub>REL_VAR - OKAY\<^esub>`"
+
+abbreviation wait_false :: 
+  "'VALUE WF_PREDICATE \<Rightarrow> 'VALUE WF_PREDICATE" ("_\<^sub>f"[150]) where
+"p\<^sub>f \<equiv> `p[false/wait]`"
 
 syntax
   "_upred_J_rea"        :: "upred" ("J\<^bsub>rea\<^esub>")
+  "_upred_wait_false"   :: "upred \<Rightarrow> upred" ("_\<^sub>f" [1000] 1000)
 
 translations
-  "_upred_J_rea"          == "CONST J_pred_rea"
+  "_upred_J_rea"        == "CONST J_pred_rea"
+  "_upred_wait_false p" == "CONST wait_false p"
 
-definition CSP1 :: "'a UTYPE \<Rightarrow> 'a WF_PREDICATE \<Rightarrow> 'a WF_PREDICATE" where
-"CSP1 a P = `P \<or> (\<not> ok \<and> (tr\<^bsub>a\<^esub> \<le> tr\<^bsub>a\<^esub>\<acute>))`"
+definition CSP1 :: "'a WF_PREDICATE \<Rightarrow> 'a WF_PREDICATE" where
+"CSP1 P = `P \<or> (\<not> ok \<and> ($tr \<le> $tr\<acute>))`"
 
-definition CSP2 :: "'a UTYPE \<Rightarrow> 'a WF_PREDICATE \<Rightarrow> 'a WF_PREDICATE" where
-"CSP2 a P = `P ; J\<^bsub>rea\<^esub>`"
+definition CSP2 :: "'a WF_PREDICATE \<Rightarrow> 'a WF_PREDICATE" where
+"CSP2 P = `P ; J\<^bsub>rea\<^esub>`"
 
-definition \<delta> :: "'a UTYPE \<Rightarrow> 'a WF_PREDICATE" where
-"\<delta> a = R3 a `((tr\<^bsub>a\<^esub> = tr\<^bsub>a\<^esub>\<acute>) \<and> $wait\<acute>)`"
-
-syntax 
-  "_upred_delta" :: "'a UTYPE \<Rightarrow> upred" ("\<delta>\<^bsub>_\<^esub>")
-
-translations
-  "_upred_delta a" == "CONST \<delta> a"
-
-definition STOP :: "'a UTYPE \<Rightarrow> 'a WF_PREDICATE" ("STOP\<^bsub>CSP'(_')\<^esub>") where
-"STOP\<^bsub>CSP(a)\<^esub> = CSP1 a `ok\<acute> \<and> \<delta>\<^bsub>a\<^esub>`"
-
-syntax 
-  "_upred_STOP" :: "'a UTYPE \<Rightarrow> upred" ("STOP\<^bsub>CSP'(_')\<^esub>")
+syntax
+  "_upred_CSP1"  :: "upred \<Rightarrow> upred" ("CSP1'(_')")
+  "_upred_CSP2"  :: "upred  \<Rightarrow> upred" ("CSP2'(_')")
 
 translations
-  "_upred_STOP a" == "CONST STOP a"
+  "_upred_CSP1 P"   == "CONST CSP1 P"
+  "_upred_CSP2 P"   == "CONST CSP2 P"
 
-definition B :: "'a UTYPE \<Rightarrow> 'a WF_PREDICATE" where
-"B a = `(tr\<^bsub>a\<^esub> = tr\<^bsub>a\<^esub>\<acute> \<and> $wait\<acute>) \<or> (tr\<^bsub>a\<^esub> \<le> tr\<^bsub>a\<^esub>\<acute>) `"
+lemma CSP_Closure : "P is (CSP1 \<circ> CSP2) \<longleftrightarrow> P = `R(\<not> P\<^sup>f\<^sub>f \<turnstile> P\<^sup>t\<^sub>f)`"
+oops 
 
-syntax 
-  "_upred_B" :: "'a UTYPE \<Rightarrow> upred" ("B\<^bsub>CSP'(_')\<^esub>")
+lemma CSP_Assignment : "`R((x :: 'a VAR):= e)` is (CSP1 \<circ> CSP2)"
+oops
 
+definition assignment :: "'a VAR \<Rightarrow> 'a WF_EXPRESSION \<Rightarrow> 'a WF_PREDICATE" ("_:=\<^bsub>CSP\<^esub>_")where
+"x:=\<^bsub>CSP\<^esub>e =`R(x:=e)`"
+
+definition deadlock :: "'a WF_PREDICATE" ("STOP") where
+"STOP = `CSP1( ok\<acute> \<and> \<delta>)`"
+
+definition prefix :: "'a WF_EXPRESSION \<Rightarrow>  'a WF_PREDICATE" ("_\<rightarrow>SKIP") where
+"a\<rightarrow>SKIP = `CSP1(ok\<acute> \<and> doA(a))`"
+
+definition SkipCSP :: "'a WF_PREDICATE" ("SKIP") where 
+"SKIP = `R(true \<turnstile> (\<exists> ref . II\<^bsub>rea\<^esub>))`"
+
+definition ChaosCSP :: "'a WF_PREDICATE" ("CHAOS") where
+"CHAOS = `R(true)`"
+
+syntax
+  "_upred_deadlock" :: "upred" ("STOP")
+  "_upred_prefix" :: "uexpr \<Rightarrow> upred" ("_\<rightarrow>SKIP")
+  "_upred_skip" :: "upred" ("SKIP")
+  "_upred_chaos" :: "upred" ("CHAOS")
+  
 translations
-  "_upred_B a" == "CONST B a"
+  "_upred_deadlock" == "CONST deadlock"
+  "_upred_prefix a" == "CONST prefix a"
+  "_upred_skip" == "CONST SkipCSP"
+  "_upred_chaos" == "CONST ChaosCSP"
 
-definition \<Phi> :: "'a UTYPE \<Rightarrow> 'a WF_PREDICATE \<Rightarrow> 'a WF_PREDICATE" where
-"\<Phi> a P = R a `B\<^bsub>CSP(a)\<^esub> \<and> P`"
+lemma L1 : "`CHAOS ; P` = `CHAOS`"
+oops
 
-definition doA :: "'a UTYPE \<Rightarrow> 'a WF_EXPRESSION \<Rightarrow> 'a WF_PREDICATE" where
-"doA a b = \<Phi> a `((b \<notin> ref\<^bsub>a\<^esub>\<acute>)\<lhd> $wait \<rhd> (tr\<^bsub>a\<^esub>^\<langle>b\<rangle> = tr\<^bsub>a\<^esub>\<acute>))`"
+lemma L2 : "`STOP ; P` = `STOP`"
+oops
 
-syntax 
-  "_upred_B" :: "'a UTYPE \<Rightarrow> 'a WF_EXPRESSION \<Rightarrow> upred" ("doA\<^bsub>CSP'(_')\<^esub>'(_')")
+definition prefixed :: "'a WF_EXPRESSION \<Rightarrow> 'a WF_PREDICATE \<Rightarrow> 'a WF_PREDICATE" ("_\<rightarrow>_") where
+"a\<rightarrow>P = `a\<rightarrow>SKIP ; P`"
 
+definition extchoice :: "'a WF_PREDICATE \<Rightarrow> 'a WF_PREDICATE \<Rightarrow> 'a WF_PREDICATE" ("_\<box>_") where
+"P\<box>Q = `CSP2((P \<and> Q)\<lhd> (($tr = $tr\<acute>) \<and> $wait\<acute>) \<rhd>(P \<or> Q))`"
+
+syntax
+  "_upred_prefixed" :: "uexpr \<Rightarrow> upred \<Rightarrow> upred" ("_\<rightarrow>_")
+  "_upred_extchoice" :: "upred \<Rightarrow> upred \<Rightarrow> upred" ("_\<box>_")
+  
 translations
-  "_upred_B a b" == "CONST doA a b"
+  "_upred_prefixed a P" == "CONST prefixed a P"
+  "_upred_extchoice P Q" == "CONST extchoice P Q"
 
-definition prefix :: "'a WF_EXPRESSION \<Rightarrow> 'a UTYPE \<Rightarrow> 'a WF_PREDICATE" ("_\<rightarrow>\<^bsub>CSP'(_')\<^esub>SKIP") where
-"a\<rightarrow>\<^bsub>CSP(b)\<^esub>SKIP = CSP1 b `ok\<acute> \<and> doA\<^bsub>CSP(b)\<^esub>(a)`"
-
-definition SkipCSP :: "'a UTYPE \<Rightarrow> 'a WF_PREDICATE" ("SKIP\<^bsub>CSP'(_')\<^esub>") where 
-"SKIP\<^bsub>CSP(a)\<^esub> = `\<exists> ref a. II\<^bsub>rea(a)\<^esub>`"
-
-definition ChaosCSP :: "'a UTYPE \<Rightarrow> 'a WF_PREDICATE" ("CHAOS\<^bsub>CSP'(_')\<^esub>") where
-"CHAOS\<^bsub>CSP(a)\<^esub> = R a true"
-
-lemma L1 : "CHAOS\<^bsub>CSP(a)\<^esub> ; P = CHAOS\<^bsub>CSP(a)\<^esub>"
+lemma L3 : "(P \<sqinter> Q) \<box> S = (P \<box> S) \<sqinter> (Q \<box> s)"
 oops
 
-lemma L2 : "STOP\<^bsub>CSP(a)\<^esub> ; P = STOP\<^bsub>CSP(a)\<^esub>"
+lemma L4 : "P \<sqinter> (Q \<box> S) = (P \<sqinter> Q) \<box> (P \<sqinter> S)"
 oops
 
-definition prefixed :: "'a WF_EXPRESSION \<Rightarrow> 'a UTYPE \<Rightarrow> 'a WF_PREDICATE \<Rightarrow> 'a WF_PREDICATE" ("_\<rightarrow>\<^bsub>CSP'(_')\<^esub>_") where
-"a\<rightarrow>\<^bsub>CSP(b)\<^esub>P = a\<rightarrow>\<^bsub>CSP(b)\<^esub>SKIP ; P"
-
-definition extchoice :: "'a WF_PREDICATE \<Rightarrow> 'a UTYPE \<Rightarrow> 'a WF_PREDICATE \<Rightarrow> 'a WF_PREDICATE" ("_\<box>\<^bsub>CSP'(_')\<^esub>_") where
-"P\<box>\<^bsub>CSP(a)\<^esub>Q = CSP2 a `((P \<and> Q)\<lhd> ((tr\<^bsub>a\<^esub> = tr\<^bsub>a\<^esub>\<acute>) \<and> $wait\<acute>) \<rhd>(P \<or> Q))`"
-
-lemma L3 : "(P \<sqinter> Q) \<box>\<^bsub>CSP(a)\<^esub> S = (P \<box>\<^bsub>CSP(a)\<^esub> S) \<sqinter> (Q \<box>\<^bsub>CSP(a)\<^esub> s)"
+lemma L5 : "`P \<box> SKIP` \<sqsubseteq> `SKIP` "
 oops
 
-lemma L4 : "P \<sqinter> (Q \<box>\<^bsub>CSP(a)\<^esub> S) = (P \<sqinter> Q) \<box>\<^bsub>CSP(a)\<^esub> (P \<sqinter> S)"
-oops
-
-lemma L5 : "P \<box>\<^bsub>CSP(a)\<^esub> SKIP\<^bsub>CSP(a)\<^esub> \<sqsubseteq> SKIP\<^bsub>CSP(a)\<^esub> "
-oops
-
-lemma L6sub : "((a1\<rightarrow>\<^bsub>CSP(a)\<^esub>P1) \<box>\<^bsub>CSP(a)\<^esub>  (a2\<rightarrow>\<^bsub>CSP(a)\<^esub>P2)); Q = ((a1\<rightarrow>\<^bsub>CSP(a)\<^esub>P1);Q) \<box>\<^bsub>CSP(a)\<^esub> ((a2\<rightarrow>\<^bsub>CSP(a)\<^esub>P2) ; Q)"
+lemma L6sub : "`((a1\<rightarrow>P1) \<box> (a2\<rightarrow>P2)); Q` = `(a1\<rightarrow>(P1;Q)) \<box> (a2\<rightarrow>(P2;Q))`"
 oops
 
 end
