theories/theories/utp_reactive.thy
@@ -12,44 +12,53 @@ imports
   utp_theory
 begin
 
-class REACTIVE_SORT = BOOL_SORT + LIST_SORT + FSET_SORT + STRING_LIST_SORT + MINUS_SORT
+class REACTIVE_SORT = BOOL_SORT + LIST_SORT + FSET_SORT + STRING_LIST_SORT + MINUS_SORT + EVENT_SORT
 
 default_sort REACTIVE_SORT
 
 abbreviation "wait \<equiv> MkPlain ''wait'' (BoolType) True"
-abbreviation tr :: "'a UTYPE \<Rightarrow> 'a::REACTIVE_SORT VAR" where
-"tr a \<equiv> MkPlain ''tr'' (ListType a) True"
+abbreviation tr :: "'a::REACTIVE_SORT VAR" where
+"tr \<equiv> MkPlain ''tr'' (ListType EventType) True"
 
-abbreviation ref :: "'a UTYPE \<Rightarrow> 'a::REACTIVE_SORT VAR" where
-"ref a \<equiv> MkPlain ''ref'' (FSetType a) True"
+abbreviation ref :: "'a::REACTIVE_SORT VAR" where
+"ref \<equiv> MkPlain ''ref'' (FSetType EventType) True"
 
-definition SkipREA :: "'a UTYPE \<Rightarrow> 'a WF_PREDICATE" where
-"SkipREA a = `(\<not> ok \<and> ($tr a \<le> $(tr a)\<acute>)) \<or> (ok\<acute> \<and> II\<^bsub>REL_VAR - OKAY\<^esub>)`"
+definition SkipREA :: "'a WF_PREDICATE" where
+"SkipREA = `(\<not> ok \<and> ($tr \<le> $tr\<acute>)) \<or> (ok\<acute> \<and> II\<^bsub>REL_VAR - OKAY\<^esub>)`"
 
 syntax 
-  "_upred_skiprea" :: "'a UTYPE \<Rightarrow> upred" ("II\<^bsub>rea'(_')\<^esub>")
-  "_upred_tr"      :: "'a UTYPE \<Rightarrow> uexpr" ("tr\<^bsub>_\<^esub>")
-  "_upred_ref"     :: "'a UTYPE \<Rightarrow> uexpr" ("ref\<^bsub>_\<^esub>")
+  "_upred_skiprea" :: " upred" ("II\<^bsub>rea\<^esub>")
 
 translations
-  "_upred_skiprea a" == "CONST SkipREA a"
-  "_upred_tr a" == "CONST VarE (CONST tr a)"
-  "_upred_ref a" == "CONST VarE (CONST ref a)"
+  "_upred_skiprea" == "CONST SkipREA"
 
 text {* R1 ensures that the trace only gets longer *}
 
-definition R1 :: "'a UTYPE \<Rightarrow> 'a WF_PREDICATE \<Rightarrow> 'a WF_PREDICATE" where
-"R1 a P = `P \<and> (tr\<^bsub>a\<^esub> \<le> tr\<^bsub>a\<^esub>\<acute>)`"
+definition R1 :: " 'a WF_PREDICATE \<Rightarrow> 'a WF_PREDICATE" where
+"R1 P = `P \<and> ($tr \<le> $tr\<acute>)`"
 
 text {* R2 ensures that the trace only gets longer *}
 
-definition R2 :: "'a UTYPE \<Rightarrow> 'a WF_PREDICATE \<Rightarrow> 'a WF_PREDICATE" where
-"R2 a P = `P[\<langle>\<rangle> / tr a][(tr\<^bsub>a\<^esub>\<acute> - tr\<^bsub>a\<^esub>) / (tr a)\<acute>]`"
+definition R2 :: "'a WF_PREDICATE \<Rightarrow> 'a WF_PREDICATE" where
+"R2 P = `P[\<langle>\<rangle> / tr][($tr\<acute> - $tr) / tr\<acute>]`"
 
-definition R3 :: "'a UTYPE \<Rightarrow> 'a WF_PREDICATE \<Rightarrow> 'a WF_PREDICATE" where
-"R3 a P = `II\<^bsub>rea(a)\<^esub> \<lhd> $wait \<rhd> P`"
+definition R3 :: "'a WF_PREDICATE \<Rightarrow> 'a WF_PREDICATE" where
+"R3 P = `II\<^bsub>rea\<^esub> \<lhd> $wait \<rhd> P`"
 
-abbreviation "R a \<equiv> R1 a \<circ> R2 a \<circ> R3 a"
+definition R :: "'a WF_PREDICATE \<Rightarrow> 'a WF_PREDICATE" where 
+"R P = (R1 \<circ> R2 \<circ> R3)P"
+
+syntax 
+  "_upred_R1" :: "upred \<Rightarrow> upred" ("R1'(_')")
+  "_upred_R2" :: "upred \<Rightarrow> upred" ("R2'(_')")
+  "_upred_R3" :: "upred \<Rightarrow> upred" ("R3'(_')")
+  "_upred_R" :: "upred \<Rightarrow> upred" ("R'(_')")
+
+translations
+  "_upred_R1 P" == "CONST R1 P"
+  "_upred_R2 P" == "CONST R2 P"
+  "_upred_R3 P" == "CONST R3 P"
+  "_upred_R P" == "CONST R P"
 
 syntax
   "_uexpr_subste"       :: "uexpr \<Rightarrow> uexpr \<Rightarrow> 'a VAR \<Rightarrow> uexpr" ("(_[_'/_])" [999,999] 1000)
@@ -62,28 +71,29 @@ lemma SubstP_ExprP [usubst]:
   by (utp_pred_tac, utp_expr_tac)
 
 lemma SkipREA_CondR_SkipR: 
-  "`II\<^bsub>rea(a)\<^esub>` = `II \<lhd> ok \<rhd> (tr\<^bsub>a\<^esub> \<le> tr\<^bsub>a\<^esub>\<acute>)`"
+  "`II\<^bsub>rea\<^esub>` = `II \<lhd> ok \<rhd> ($tr \<le> $tr\<acute>)`"
 proof -
 
-  have "`II \<lhd> ok \<rhd> (tr\<^bsub>a\<^esub> \<le> tr\<^bsub>a\<^esub>\<acute>)` = `($okay\<acute> = $okay \<and> II\<^bsub>REL_VAR - OKAY\<^esub>) \<lhd> ok \<rhd> (tr\<^bsub>a\<^esub> \<le> tr\<^bsub>a\<^esub>\<acute>)`"
+  have "`II \<lhd> ok \<rhd> ($tr \<le> $tr\<acute>)` = `($okay\<acute> = $okay \<and> II\<^bsub>REL_VAR - OKAY\<^esub>) \<lhd> ok \<rhd> ($tr \<le> $tr\<acute>)`"
     by (metis Diff_cancel ExistsP_empty HOMOGENEOUS_REL_VAR MkPlain_UNDASHED SkipRA.rep_eq SkipRA_unfold UnCI hom_alphabet_undash)
 
-  also have "... = `($okay\<acute> = $okay \<and> II\<^bsub>REL_VAR - OKAY\<^esub>)[true/okay] \<lhd> $okay \<rhd> ((tr\<^bsub>a\<^esub> \<le> tr\<^bsub>a\<^esub>\<acute>)[false/okay])`"
+  also have "... = `($okay\<acute> = $okay \<and> II\<^bsub>REL_VAR - OKAY\<^esub>)[true/okay] \<lhd> $okay \<rhd> (($tr \<le> $tr\<acute>)[false/okay])`"
     by (rule CondR_VarP_aux, simp_all add:typing defined)
 
-  also have "... = `(ok \<and> II\<^bsub>REL_VAR - OKAY\<^esub>) \<lhd> ok \<rhd> (tr\<^bsub>a\<^esub> \<le> tr\<^bsub>a\<^esub>\<acute>)`"
+  also have "... = `(ok \<and> II\<^bsub>REL_VAR - OKAY\<^esub>) \<lhd> ok \<rhd> ($tr \<le> $tr\<acute>)`"
   proof -
-
+(*
     have "(ulesseq :: 'b \<Rightarrow> 'b \<Rightarrow> 'b) \<in> FUNC2 (ListType StringType) (ListType StringType) BoolType"
       by (simp add: closure) 
 
     thus ?thesis
-(*
+
       apply (insert SubstE_Op2E[of "VarE tr :: 'b WF_EXPRESSION" "ListType StringType" "VarE tr\<acute>" "ListType StringType" "ulesseq" BoolType "FalseE" "okay"])
 
     apply (simp add:usubst typing defined closure var_simps)
 *)
 
   oops (* FIXME: Can't finish the step without more laws about prefix *)
+
 
 end
