theories/theories/utp_acp.thy
@@ -1,0 +1,67 @@
+(******************************************************************************)
+(* Project: Mechanisation of the UTP                                          *)
+(* File: utp_csp.thy                                                          *)
+(* Authors: Samuel Canham and Simon Foster, University of York                *)
+(******************************************************************************)
+
+header {* ACP Processes *}
+
+theory utp_acp
+imports 
+  utp_designs
+  utp_theory
+  utp_reactive
+begin
+
+definition ACP1 :: "'a WF_PREDICATE \<Rightarrow> 'a WF_PREDICATE" where
+"ACP1 P = `P \<and> (($tr = $tr\<acute>) \<Rightarrow> $wait)` "
+
+definition \<delta> :: "'a WF_PREDICATE" where
+"\<delta> = `R3($tr = $tr\<acute> \<and> $wait\<acute>)`"
+
+definition B :: "'a WF_PREDICATE" where
+"B = `($tr = $tr\<acute> \<and> $wait\<acute>) \<or> ($tr \<le> $tr\<acute>)`"
+
+definition \<Phi> :: "'a WF_PREDICATE \<Rightarrow> 'a WF_PREDICATE" where
+"\<Phi>(P) = `R(B \<and> P)`"
+
+syntax 
+  "_upred_Phi" :: "upred \<Rightarrow> upred" ("\<Phi>'(_')")
+
+translations
+  "_upred_Phi P" == "CONST \<Phi> P"
+
+definition doA :: "'a WF_EXPRESSION \<Rightarrow> 'a WF_PREDICATE" where
+"doA(a) = `\<Phi>(a \<notin> $ref\<acute>\<lhd> $wait \<rhd> ($tr^\<langle>a\<rangle> = $tr\<acute>))`"
+
+syntax 
+  "_upred_doA" :: "uexpr \<Rightarrow> upred" ("doA'(_')")
+
+translations
+  "_upred_doA a" == "CONST doA a"
+
+lemma L1 : "\<delta> ; P = \<delta>"
+apply (simp add:\<delta>_def R3_def SkipREA_def)
+oops
+
+definition alternative :: "'a WF_PREDICATE \<Rightarrow> 'a WF_PREDICATE \<Rightarrow> 'a WF_PREDICATE" ("_ +\<^bsub>ACP\<^esub> _") where
+"(P +\<^bsub>ACP\<^esub> Q) = `(P \<and> Q)\<lhd> \<delta> \<rhd> (P \<or> Q)`"
+
+lemma L2 : "P +\<^bsub>ACP\<^esub> P = P"
+oops
+
+lemma L3 : "P +\<^bsub>ACP\<^esub> Q = Q +\<^bsub>ACP\<^esub> P"
+oops
+
+lemma L4 : "(P +\<^bsub>ACP\<^esub> Q)+\<^bsub>ACP\<^esub> S = P +\<^bsub>ACP\<^esub> (Q +\<^bsub>ACP\<^esub> S)"
+oops
+
+lemma L5 : "\<delta> +\<^bsub>ACP\<^esub> Q = Q"
+oops
+
+lemma L6 : "(P +\<^bsub>ACP\<^esub> Q) ; S = (P;S) +\<^bsub>ACP\<^esub> (Q;S)"
+oops
+
+
+
+end
